{
 "cells": [
  {
   "cell_type": "markdown",
   "metadata": {},
   "source": [
    "# 03 Nonhomogeneous Poisson Process\n",
    "\n",
    "## Nonhomogeneous Poisson Process\n",
    "\n",
    "Nonhomogeneous Poisson process (NHPP) has variant rate parameter $\\lambda$. Its \"rare event\" property is redefined by\n",
    "\n",
    "$$\\begin{aligned}\\mathbb P\\left(N(t+\\Delta t) - N(t)=1\\right) &= \\lambda(t)\\cdot\\Delta t + o(\\Delta t)\n",
    "\\\\ \\mathbb P\\left(N(t+\\Delta t) - N(t)\\geqslant 2\\right) &=  o(\\Delta t)\n",
    "\\end{aligned}$$\n",
    "\n",
    "Here $\\lambda(t)$ is a function of $t$.\n",
    "\n",
    "It therefore no longer preserves stationary increments. But we still require independent increments. \n",
    "\n",
    "**Theorem** If we define $m(s,t)=\\int_s^t \\lambda (u)du$, we have\n",
    "\n",
    "$$\\mathbb P(N(s,t]=k)  = \\frac{m(s,t)^{k}}{k!}e^{-m(s,t)}.$$\n",
    "\n",
    "**Proof** Denote $P_k(t) = P(N(t)=k)$. Note that $P_0(0)=1$. Then we have\n",
    "$$\\begin{aligned}P_0(t+\\Delta t) &= P(N(t+\\Delta t) = 0)=\\mathbb P(N(t)=0,\\ N(t+\\Delta t)-N(t)=0)\n",
    "\\\\ &= \\mathbb P(N(t)=0)\\cdot \\mathbb P(N(t,t+\\Delta t]=0)\n",
    "\\\\ &= P_0(t)\\cdot (1 -\\lambda (t)\\Delta t+o(\\Delta t)).\n",
    "\\end{aligned}$$\n",
    "\n",
    "Thus we see that $\\mathbb P_0'(t) = -\\lambda(t)P_0(t)$ by the definition of derivative, which has solution $P_0(t) = e^{-m(0,t)}$. Similarly, we have\n",
    "$$\\begin{aligned}P_k(t+\\Delta t)& = \\mathbb P(N(t)=k)\\cdot \\mathbb P(N(t,t+\\Delta t]=0)+\\mathbb P(N(t)=k-1)\\cdot \\mathbb P(N(t,t+\\Delta t]=1)+o(\\Delta t)\n",
    "\\\\ &= P_k(t)+\\left(-P_k(t)+ P_{k-1}(t)\\right)\\lambda (t)\\cdot\\Delta t + o(\\Delta t).\n",
    "\\end{aligned}$$\n",
    "\n",
    "Then we can prove by induction that $P_k(t) = \\frac{m(0,t)^{k}}{k!}e^{-m(0,t)}$. Finally, the proof can be generalized to arbitrary initial start time $s$ so $m(0,t)$ is replaced by $m(s,t)$ for $P(N(s,t]=k)$."
   ]
  },
  {
   "cell_type": "markdown",
   "metadata": {},
   "source": [
    "## Arrival and Waiting\n",
    "\n",
    "### Arrival Time\n",
    "\n",
    "If $N(t)=k$, then there are $k$ events before time $t$. Denote $s_i$ be the occurrence time of the $i$-th event. We call it the arrival time.\n",
    "\n",
    "**Theorem** If $N(t)$ flows a nonhomogeneous Poisson process with rate $\\lambda$, then $s_n$ has P.D.F. $f_{s_n}(t) = \\frac{\\lambda(t)m(0,t)^{n-1}}{(n-1)!}e^{-m(0,t)}$.\n",
    "\n",
    "**Proof** We have\n",
    "$$\\begin{aligned}\\mathbb P(s_n\\leqslant t) &= \\mathbb P(N(t)\\geqslant n) = 1-\\sum_{k=0}^{n-1} \\frac{m(0,t)^k}{k!}e^{-m(0,t)}.\\end{aligned}$$\n",
    "\n",
    "Then we can take the derivative to get the P.D.F. of $s_n$ that\n",
    "$$\\begin{aligned}f_{s_n}(t) &= \\frac{d}{dt}\\sum_{k=n}^{\\infty} \\frac{m(0,t)^k}{k!}e^{-m(0,t)}=\n",
    "\\sum_{k=n}^{\\infty}\\frac{m(0,t)^k}{k!}\\left(\\frac{k}{m(0,t)}-1\\right)\\lambda (t)e^{-m(0,t)}=\\frac{\\lambda(t)m(0,t)^{n-1}}{(n-1)!}e^{-m(0,t)}.\\end{aligned}$$\n",
    "\n",
    "### Waiting Time\n",
    "\n",
    "The waiting time is no longer independent with each other in a nonhomogeneous Poisson process. But we can still calculate the P.D.F. of the waiting time.\n",
    "\n",
    "\n",
    "**Theorem** If $N(t)$ flows a nonhomogeneous Poisson process with rate $\\lambda$, then for $n\\geqslant 2$, the P.D.F. of the waiting time $x_n=s_n-s_{n-1}$ is given by \n",
    "\n",
    "$$f_{x_n}(t)=\\frac{1}{(n-2)!}\\int_0^\\infty \\lambda(s)m(0,s)^{n-2}e^{-m(0,s+t)} ds.$$\n",
    "\n",
    "**Proof** For $n\\geqslant 2$,\n",
    "\n",
    "$$\\begin{aligned}\\mathbb P(x_n>t) &= \\mathbb P(s_n-s_{n-1}>t) = \\int_0^\\infty \\mathbb P(s_n>t+s|s_{n-1}=s)f_{s_{n-1}}(s)ds\\\\ &=\\int_0^\\infty \\mathbb P(N(t+s) - N(s) = 0)f_{s_{n-1}}(s)ds\\\\ &=  \\int_0^\\infty {e^{-m(s,s+t)}}{ }\\cdot\\frac{\\lambda(s)m(0,s)^{n-2}}{(n-2)!}e^{-m(0,s)} ds.\\end{aligned}$$"
   ]
  },
  {
   "cell_type": "markdown",
   "metadata": {},
   "source": [
    "## Time Translation\n",
    "\n",
    "In the following, we consider a nonhomogeneous Poisson process with rate $\\lambda(t)$, denoted by $\\tilde N(t)$. We define $m(t) = \\int_0^\\infty \\lambda(s)ds$ and its inverse function to be $m^{-1}(\\cdot)$.\n",
    "\n",
    "**Theorem** Let $N(t) = \\tilde N(m^{-1}(t))$, then $N(t)$ is a homogeneous Poisson process with rate $1$.\n",
    "\n",
    "**Proof** \n",
    "\n",
    "Firstly, $N(0)= \\tilde N(0)=0$. \n",
    "\n",
    "Secondly, the \"rare event\" property is preserved by\n",
    "$$\\mathbb P(N(t+\\Delta t) -N(t)=k) = \\mathbb P\\left(\\tilde N(m^{-1}(t+\\Delta t)) - \\tilde N(m^{-1}(t))=k\\right).$$\n",
    "\n",
    "Note that $m'(t)=\\lambda (t)$, so we have $\\frac{\\partial }{\\partial t}m^{-1}(t) = \\frac{1}{\\lambda(m^{-1}(t))}$. Thus,\n",
    "\n",
    "$$\\tilde\\Delta t = m^{-1}(t+\\Delta t)-m^{-1}(t) = \\frac{1}{\\lambda (m^{-1}(t))}\\Delta t+ o(\\Delta t).$$\n",
    "\n",
    "And we have\n",
    "$$\\begin{aligned}\\mathbb P\\left(\\tilde N(m^{-1}(t+\\Delta t)) - \\tilde N(m^{-1}(t))=1\\right) &= \\lambda(m^{-1}(t))\\cdot \\tilde \\Delta t+o(\\tilde \\Delta t)=\\Delta t+ o(\\Delta t)\n",
    "\\\\  \\mathbb P\\left(\\tilde N(m^{-1}(t+\\Delta t)) - \\tilde N(m^{-1}(t))\\geqslant 2\\right) &= o(\\tilde \\Delta t)= o(\\Delta t).\\end{aligned}$$\n",
    "\n",
    "Thirdly, the stationarity is shown by $(s<t)$\n",
    "$$\\begin{aligned}\\mathbb P(N(t)-N(s)=k) &= \\mathbb P\\left(\\tilde N(m^{-1}(t)) - \\tilde N(m^{-1}(s)) = k\\right)\n",
    "\\\\ &= \\frac{m(m^{-1}(s),m^{-1}(t))^{k}}{k!}e^{-m(m^{-1}(s),m^{-1}(t))}=\\frac{(t-s)^k}{k!}e^{-(t-s)}.\n",
    "\\end{aligned}$$\n",
    "\n",
    "<!-- Finally, the independent increment property is proven with the aid of characteristic function. For fixed $s<t$, we have\n",
    "$$\\phi_{N(t)-N(s),N(s)}(a,b)=\\mathbb E\\exp\\left\\{ia(N(t)-N(s)) + ibN(s)\\right\\}$$ -->\n",
    "\n",
    "Finally, the independence of increment is shown by, for $s<t$ that,\n",
    "$$\\begin{aligned}\\mathbb P(N(t)-N(s)=k_1, N(s)=k_2) & =\\mathbb P\\left(\\tilde N(m^{-1}(t))-\\tilde N(m^{-1}(s))=k_1, \\tilde N(m^{-1}(s))=k_2\\right)\\\\ & =\\mathbb P\\left(\\tilde N(m^{-1}(t))-\\tilde N(m^{-1}(s))=k_1\\right)\\mathbb P\\left(\\tilde N(m^{-1}(s))=k_2\\right).\\end{aligned}$$\n",
    "\n",
    "In the last equality we have used the fact that $\\tilde N(u) - \\tilde N(v)$ and $\\tilde N(v)$ are independent."
   ]
  },
  {
   "cell_type": "markdown",
   "metadata": {},
   "source": [
    "## Compound Poisson Process\n",
    "\n",
    "Assume $N(t)$ is a homogeneous Poisson process with rate $\\lambda$. Suppose $\\xi_1,\\xi_2,\\dotsc$ are i.i.d. random variables and they are all independent with $N(t)$. Define $Z(t) = \\sum_{i=1}^{N(t)}\\xi_i$. Then $Z(t)$ is called a compound Poisson process.\n",
    "\n",
    "### Examples\n",
    "\n",
    "For example, the number of customers arriving in a shop can be simulated by a Poisson process. And the total amount of money they spend can be simulated by a compound Poisson process.\n",
    "\n",
    "As for another example, let $\\xi_i\\sim B(p)$ is Bernoulli distributed. Then $Z(t)$ is the number of times that a Bernoulli trial is successful, which is a decomposition of the Poisson process.\n",
    "\n",
    "\n",
    "### Properties\n",
    "\n",
    "Aside from $Z(0)=0$, compound Poisson process $Z(t)$ has independent and stationary increments.\n",
    "\n",
    "#### Independent Increments\n",
    "\n",
    "**Theorem** for $s<t$, $Z(t)-Z(s)$ is independent with $Z(s)$.\n",
    "\n",
    "**Proof** Using the method of characteristic function, we have\n",
    "\n",
    "$$\\begin{aligned}\\phi_{Z(t)-Z(s),Z(s)}(a,b) &= \\mathbb E\\exp\\left\\{ia(Z(t)-Z(s))+ibZ(s)\\right\\}\n",
    "\\\\ &= \\mathbb E_{N(t),N(s)}\\mathbb E_{\\xi}\\exp\\left\\{ia(Z(t)-Z(s))+ibZ(s)\\right\\}\n",
    "\\\\ &= \\mathbb E_{N(t),N(s)}\\mathbb E_{\\xi}\\exp\\left\\{ia\\sum_{k>N(s)}^{N(t)}\\xi_k+ib\\sum_{k=1}^{N(s)}\\xi_k\\right\\}\\\\ &= \\mathbb E_{N(t),N(s)}\\left\\{\\phi_\\xi(a)^{N(t)-N(s)}\\phi_\\xi(b)^{N(s)}\\right\\}\\\\ &= \\mathbb E_{N(t-s),N(s)}\\left\\{\\phi_\\xi(a)^{N(t-s)}\\phi_\\xi(b)^{N(s)}\\right\\}\n",
    "\\\\ &= \\mathbb E_{N(t-s)}\\left\\{\\phi_\\xi(a)^{N(t-s)}\\right\\}\\mathbb E_{N(s)}\\left\\{\\phi_\\xi(b)^{N(s)}\\right\\}.\n",
    "\\end{aligned} $$\n",
    "\n",
    "It is in the form of $f_1(a)f_2(b)$, which means $Z(t)-Z(s)$ is independent with $Z(s)$.\n",
    "\n",
    "#### Stationary Increments\n",
    "\n",
    "**Theorem** For $s<t$, $Z(t)-Z(s)$ has the same distribution as $Z(t-s)$.\n",
    "\n",
    "**Proof** Using the method of characteristic function combined with the details above,\n",
    "\n",
    "$$\\phi_{Z(t)-Z(s)}(a) = \\mathbb E\\exp\\left\\{ia(Z(t)-Z(s))\\right\\} = \\mathbb E_{N(t-s)}\\left\\{\\phi_\\xi(a)^{N(t-s)}\\right\\}.$$\n",
    "\n",
    "It only depends on $t-s$, so $Z(t)-Z(s)$ has the same distribution as $Z(t-s)-Z(0)=Z(t-s)$.\n",
    "\n",
    "\n",
    "### Statistics\n",
    "\n",
    "Now we assume the original Poisson process $N(t)$ has rate $\\lambda$ and $\\xi_i$ has mean $\\mu$ and variance $\\sigma^2$. \n",
    "\n",
    "**Theorem** $\\mathbb E(Z(t)) = \\lambda t\\mu$ and ${\\rm Var}(Z(t))=\\lambda t(\\mu^2 +\\sigma^2)$.\n",
    "\n",
    "**Proof** The mean is given by\n",
    "\n",
    "$$\\mathbb E(Z(t)) = \\mathbb E_{N(t)}\\mathbb E_\\xi \\sum_{i=1}^{N(t)}\\xi_i = \\mathbb E_{N(t)}N(t)\\mu = \\lambda t\\mu.$$\n",
    " \n",
    "To compute the variance, we first compute the second moment\n",
    "\n",
    "$$\\begin{aligned}\\mathbb E(Z^2(t)) &= \\mathbb E_{N(t)}\\mathbb E_\\xi \\left(\\sum_{i=1}^{N(t)}\\xi_i\\right)^2\n",
    "=\\mathbb E_{N(t)}\\left\\{N(t)(\\mu^2+\\sigma^2)+N(t)(N(t)-1)\\mu^2\\right\\} \n",
    "\\\\ &= \\lambda t(\\mu^2+\\sigma^2)+(\\lambda^2t^2+\\lambda t-\\lambda t)\\mu^2=\\lambda t(\\mu^2+\\sigma^2)+\n",
    "\\lambda^2t^2\\mu^2.\n",
    "\\end{aligned}$$\n",
    "\n",
    "Therefore the variance is the difference between the second moment and the square of the mean, which is $\\lambda t(\\mu^2+\\sigma^2)$.\n",
    "\n",
    "<br>\n",
    "\n",
    "NOTE: Since the Poisson process requires the mean and the variance are equal, we can see that the compound Poisson process is generally NOT a Poisson process.\n",
    "\n",
    "\n",
    "#### Characteristic Function\n",
    "\n",
    "**Theorem** The characteristic function of $Z(t)$ is given by $\\phi_{Z(t)}(a)=\\exp\\left\\{\\lambda t\\left(\\phi_{\\xi}(a)-1\\right)\\right\\}$.\n",
    "\n",
    "**Proof** \n",
    "\n",
    "$$\\begin{aligned}\\phi_{Z(t)}(a)&= \\mathbb E \\exp\\left\\{ia\\sum_{k=1}^{N(t)}  \\xi_k\\right\\}=\\mathbb E_{N(t)} \\mathbb E_\\xi\\exp\\left\\{ia\\sum_{k=1}^{N(t)}  \\xi_k\\right\\}\n",
    " = \\mathbb E_{N(t)}\\left\\{\\phi_{\\xi}(a)^{N(t)} \\right\\}\n",
    " \\\\ &= \\sum_{k=0}^\\infty \\frac{(\\lambda t)^k}{k!}e^{-\\lambda t}\\phi_{\\xi}(a)^{k} = \\exp\\left\\{\\lambda t\\left(\\phi_{\\xi}(a)-1\\right)\\right\\}.\n",
    "\\end{aligned}$$"
   ]
  }
 ],
 "metadata": {
  "language_info": {
   "name": "python"
  }
 },
 "nbformat": 4,
 "nbformat_minor": 2
}
