{
 "cells": [
  {
   "attachments": {},
   "cell_type": "markdown",
   "metadata": {},
   "source": [
    "# 5 Generalized Linear Model \n",
    "\n",
    "## Least Squares\n",
    "\n",
    "Assume $y\\sim (X\\beta, \\sigma^2 I)$ with $\\beta\\in\\mathbb R^{k+1},\\ X\\in\\mathbb R^{n\\times (k+1)},\\ y\\in\\mathbb R^n$ is a linear model with $n$ data. Assume $X$ is of full rank and known (we call $X$ the design matrix). Now $y$ is observed and we want to estimate $\\beta$, it is then well-known that the MSE estimator gives $\\hat\\beta = (X^TX)^{-1}X^Ty$.\n",
    "\n",
    "#### Orthogonality\n",
    "\n",
    "$y - X\\hat\\beta$ and $X\\hat\\beta$ are orthogonal.\n",
    "\n",
    "**Proof** Use $X^TX\\hat\\beta = X^Ty$ (which also holds even when $X$ is not of full rank):\n",
    "\n",
    "$$(y - X\\hat\\beta)^T X\\hat\\beta = y^TX\\hat\\beta - \\hat\\beta^T(X^TX\\hat\\beta)= y^TX\\hat\\beta -\\hat\\beta^TX^Ty = 0.$$\n",
    "\n",
    "\n",
    "#### Gauss Markov Theorem\n",
    "\n",
    "**Theorem** Assume $y= X\\beta+\\epsilon$ where noise $\\epsilon$ is mean-zero, uncorrelated and homoscedastic with variance $\\sigma^2$. Then $\\hat\\beta = (X^TX)^{-1}X^Ty$ is the BLUE (best linear unbiased estimator).\n",
    "\n",
    "**Proof** Assume the BLUE is $\\hat\\beta^* = Ay+b$. Since it should be unbiased, we require $\\beta = \\mathbb E\\hat\\beta^* = \\mathbb E(Ay+b) = AX\\beta +b$ for all $\\beta$. Scaling $\\beta$ shows that $b\\equiv 0$ and then $AX = I$. If we write $A = (X^TX)^{-1}X^T +D $, then $DX =0$. Now we check the variance matrix of $\\hat\\beta^*$, \n",
    "\n",
    "$${\\rm Var}\\hat\\beta^* = {\\rm Var}Ay = \\sigma^2 AA^T = \\sigma^2\\left[ (X^TX)^{-1}+DD^T\\right]\\succeq \\sigma^2(X^TX)^{-1}.$$\n",
    "\n",
    "The minimum is reached if and only if $D = 0$ and $A = (X^TX)^{-1}X^Ty$, which is exactly $\\hat\\beta = (X^TX)^{-1}X^Ty$."
   ]
  },
  {
   "attachments": {},
   "cell_type": "markdown",
   "metadata": {},
   "source": [
    "## Generalized Linear Model \n",
    "\n",
    "Recall we can treat the least squares model as an optimization problem in the **parametric family**:\n",
    "\n",
    "$$y_i \\sim N(x_i^T\\beta, \\sigma^2)\\quad\\quad\\quad x_i^T\\in\\mathbb R^{k+1},$$\n",
    "\n",
    "or, in the form of p.d.f.,\n",
    "\n",
    "$$f_{\\beta,\\sigma^2}(y_i) = \\frac{1}{\\sqrt{2\\pi\\sigma^2 }}\\exp\\left\\{-\\frac{1}{2\\sigma^2}(y_i - x_i^T\\beta)^2\\right\\}$$\n",
    "\n",
    "with $\\beta$ and $\\sigma^2$ are unknown parameters. It is also an exponential family. The least squares problem is finding the parameters $(\\beta,\\sigma^2)$ that maximize the joint likelihood of the observations.\n",
    "\n",
    "<br>\n",
    "\n",
    "In general, generalized linear model (GLM) takes the following form: modelling the observation by a parametric family $(\\phi>0)$ with p.d.f. given below\n",
    "\n",
    "$$f_{\\beta,\\phi}(y_i)= h(y_i,\\phi) \\exp\\left\\{\\frac{y_i\\eta_i - \\zeta(\\eta_i) }{\\phi} \\right\\},\\quad\\quad \\eta_i=\\eta(\\beta^Tx_i)$$\n",
    "\n",
    "Here $\\beta,\\phi$ are unknown parameters for the family while $x_i$ are known parameters (coeffcients). $h,\\zeta,\\eta$ are functions. The family is not an exponential family. However, <font color=red>it is an exponential family when treating</font> $\\phi$ <font color=red>as a constant.</font>\n",
    "\n",
    "\n",
    "### Linear and Logistic Examples\n",
    "\n",
    "Linear model is a special case of the generalized linear model, as long as we take $\\phi =\\sigma^2$ and $h(y_i,\\phi)=\\frac{1}{\\sqrt{2\\pi\\sigma^2 }}\\exp \\left\\{-\\frac{y_i^2}{2\\sigma^2}\\right\\}$ and $\\zeta(\\eta) = \\frac12\\eta^2$ and $\\eta(z)=z$. In this case, $\\eta_i = \\beta^Tx_i$ and\n",
    "\n",
    "$$f_{\\beta,\\sigma^2}(y_i) = \\frac{1}{\\sqrt{2\\pi\\sigma^2 }}\\exp \\left\\{-\\frac{y_i^2}{2\\sigma^2}\\right\\}\\exp\\left\\{\\frac{ y_i (\\beta^Tx_i) -\\frac{1}{2 }(\\beta^Tx_i)^2}{\\sigma^2}\\right\\}.$$\n",
    "\n",
    "Logistic regression is also a special case. Let $p_i = \\frac{1}{1+\\exp\\{-\\beta^Tx_i\\}}$ and $\\log \\frac{p_i}{1-p_i} = \\beta^Tx_i$, then we can take $\\phi\\equiv 1$, $h(y_i,\\phi) =  \\mathbb I_{y_i\\in\\{0,1\\}}$, $\\zeta(\\eta) =- \\log (1 - \\frac{1}{1+e^{-\\eta}})=-\\log (1 - p_i)$ and $\\eta(z) = z$, such that $\\eta_i = \\beta^Tx_i$ and\n",
    "\n",
    "$$f_{\\beta}(y_i) = \\mathbb I_{y_i\\in\\{0,1\\}} p_i^{y_i}(1-p_i)^{1-y_i}\n",
    "= \\mathbb I_{y_i\\in\\{0,1\\}} \\exp\\left\\{y_i\\log \\frac{p_i}{1-p_i}+\\log (1 - p_i)\\right\\}\n",
    "= \\mathbb I_{y_i\\in\\{0,1\\}} \\exp\\left\\{y_i(x_i^T\\beta)+\\log (1 - p_i)\\right\\}.$$\n",
    "\n",
    "### Statistical Property\n",
    "\n",
    "We have $\\mathbb E(y_i) = \\zeta'(\\eta_i)$ and ${\\rm Var}(y_i) = \\phi \\zeta''(\\eta_i)$. Here $\\eta_i = \\beta^Tx_i$. Note that $\\phi$ controls the variance rather expectance, and $\\phi$ is called the dispersion parameter.\n",
    "\n",
    "**Proof** Since $\\int h(y,\\phi) \\exp\\left\\{\\frac{y\\eta_i - \\zeta(\\eta_i) }{\\phi} \\right\\}dy = 1$, we take derivative with respect to $\\eta_i$ on both sides to yield\n",
    "\n",
    "$$0 = \\frac{\\partial }{\\partial \\eta_i}\\int h(y,\\phi) \\exp\\left\\{\\frac{y\\eta_i - \\zeta(\\eta_i) }{\\phi} \\right\\}dy \n",
    "=\\int h(y,\\phi) \\exp\\left\\{\\frac{y\\eta_i - \\zeta(\\eta_i) }{\\phi} \\right\\}\\left[ \\frac{y - \\zeta'(\\eta_i)}{\\phi}\\right]dy. $$\n",
    "\n",
    "Therefore $\\mathbb E(y_i ) =\\displaystyle \\int h(y,\\phi) \\exp\\left\\{\\frac{y\\eta_i - \\zeta(\\eta_i) }{\\phi} \\right\\}y_idy = \\zeta'(\\eta_i)\\displaystyle \\int h(y,\\phi) \\exp\\left\\{\\frac{y\\eta_i - \\zeta(\\eta_i) }{\\phi} \\right\\}dy =  \\zeta'(\\eta_i) $.\n",
    "\n",
    "\n",
    "Similarly the second derivative gives\n",
    "\n",
    "$$0 =\\phi \\frac{\\partial^2 }{\\partial \\eta_i^2}\\int h(y,\\phi) \\exp\\left\\{\\frac{y\\eta_i - \\zeta(\\eta_i) }{\\phi} \\right\\}dy \n",
    "=\\int h(y,\\phi) \\exp\\left\\{\\frac{y\\eta_i - \\zeta(\\eta_i) }{\\phi} \\right\\}\\left[ -\\zeta''(\\eta_i)+\\frac{(y - \\zeta'(\\eta_i) )^2}{\\phi}\\right]dy. $$\n",
    "\n",
    "Sort the equality yields ${\\rm Var}(y_i )=\\mathbb E(y_i^2) - \\left[\\mathbb E(y_i)\\right]^2= \\phi \\zeta''(\\eta_i)$.\n",
    "\n",
    "\n",
    "\n",
    "### Link Function\n",
    "\n",
    "Define $g$ by the **inverse function** of $\\zeta'(\\eta(\\cdot))$. Call $g$ the link function. Moreover, when $\\eta (z)\\equiv z$ is the identity, we call $g$ the natural link / canonical link.\n",
    "\n",
    "For example, in linear regression $\\zeta(\\eta(z)) = \\frac12z^2$ and $\\zeta'(\\eta(z)) =z$, since $\\left[\\zeta'(\\eta(z))\\right]^{-1} = z$, so the natural link of linear regression is identity. Whilst in logistic regression, $\\zeta(\\eta) = -\\log\\left[ 1 - \\frac{1}{1+e^{-\\eta}}\\right]$ and $\\zeta'(\\eta(z)) = \\frac{1}{1+e^{-z}}$, and $g(z) = \\left[\\zeta'(\\eta(z))\\right]^{-1}= \\ln\\frac{z}{1-z}$, which is known as the logit link.\n",
    "\n",
    "It is clear that $g(\\mathbb E(y_i)) = \\beta^Tx_i$."
   ]
  },
  {
   "attachments": {},
   "cell_type": "markdown",
   "metadata": {},
   "source": [
    "\n",
    "### Maximum Likelihood Estimator\n",
    "\n",
    "For $\\phi$ being any fixed value, the MLE for parameter $\\eta$ does not depend on $\\phi$. Thus we can treat $\\phi$ as a constant and the parametric family exponential when computing the MLE for $\\beta$.\n",
    "\n",
    "**Proof** The joint log-likelihood is given by\n",
    "\n",
    "$$\\log\\ell = \\sum_{i=1}^n \\log f(y_i) = \\sum_{i=1}^n\\left[\\log h(y_i,\\phi)\n",
    "+\\frac{y_i\\eta - \\zeta(\\eta) }{\\phi}\\right]  \n",
    "=\\sum_{i=1}^n \\log h(y_i,\\phi) + \\frac{1}{\\phi} \\sum_{i=1}^n [{y_i \\eta_i - \\zeta(\\eta_i) }].$$\n",
    "\n",
    "Since $\\eta_i = \\eta(\\beta^Tx_i)$, therefore, for whatever $\\phi$, the MLE for parameter $\\beta$ is the maximizer of $\\sum_{i=1}^n [{y_i\\eta(\\beta^Tx_i) - \\zeta(\\eta(\\beta^Tx_i)) }]$.\n",
    "\n",
    "<br>\n",
    "\n",
    "Also, let\n",
    "\n",
    "$$\\begin{aligned}\n",
    "M_n(\\beta) &= \\sum_{i=1}^n  [\\eta'(\\beta^Tx_i)] ^2 \\zeta'' (\\eta_i)x_ix_i^T\n",
    "\\quad{\\rm and}\\quad R_n(\\beta)  = \\sum_{i=1}^n [y_i - \\zeta'(\\eta_i)]\\eta''(\\beta^Tx_i)x_ix_i^T.\n",
    "\\end{aligned}$$\n",
    "\n",
    "Then $\\frac{\\partial^2}{\\partial \\beta\\partial \\beta^T}\\log \\ell = [R_n(\\beta) - M_n(\\beta)] / \\phi$.\n",
    "\n",
    "**Proof**\n",
    "\n",
    "$$\\begin{aligned} \\frac{\\partial\\log\\ell}{\\partial \\beta^T} &= \\frac{1}{\\phi}\\frac{\\partial }{\\partial \\beta^T} \\sum_{i=1}^n [{y_i\\eta(\\beta^Tx_i) - \\zeta(\\eta(\\beta^Tx_i)) }]   =\\frac{1}{\\phi} \\sum_{i=1}^n\\left[  y_i\\eta'(\\beta^Tx_i)x_i^T - \\zeta' (\\eta(\\beta^Tx_i))\\eta'(\\beta^Tx_i)x_i^T\n",
    "\\right] \\\\ &  =\\frac{1}{\\phi} \\sum_{i=1}^n  [ y_i  - \\zeta' (\\eta(\\beta^Tx_i))]\\eta'(\\beta^Tx_i)x_i^T\n",
    "\\\\ \n",
    "\\frac{\\partial^2\\log\\ell}{\\partial \\beta\\partial \\beta^T} &= \\frac{1}{\\phi} \\frac{\\partial }{\\partial \\beta} \\sum_{i=1}^n  [ y_i  - \\zeta' (\\eta(\\beta^Tx_i))]\\eta'(\\beta^Tx_i)x_i^T\\\\ &=  \\frac{1}{\\phi} \\sum_{i=1}^n \\left\\{-\\zeta''(\\eta(\\beta^T(x_i)))[\\eta'(\\beta^Tx_i)]^2x_ix_i^T +  [ y_i  - \\zeta' (\\eta(\\beta^Tx_i))]\\eta''(\\beta^Tx_i)x_ix_i^T\\right\\}\n",
    " \\end{aligned}\n",
    "$$\n",
    "\n",
    "Remark: note that $\\eta'' = 0$ when $g$ is canonical, i.e. $\\eta(z) = z$, so in this case $\\frac{\\partial^2 \\log \\ell}{\\partial \\beta\\partial \\beta^T} =M_n(\\beta)/\\phi$. Further, when $\\eta(z) = z$ and $\\zeta$ is convex, we can see that $-\\log\\ell$ is also convex since $M_n(\\beta)$ is positive semidefinite."
   ]
  },
  {
   "attachments": {},
   "cell_type": "markdown",
   "metadata": {},
   "source": [
    "## Cramér Rao Lower Bound\n",
    "\n",
    "### Fisher Information Matrix\n",
    "\n",
    "Suppose all distributions of a parametric family $\\mathcal P$ has p.d.f $f_\\theta\\ (\\theta\\in\\Theta)$ (on measure $\\nu$). Then we define the Fisher information matrix to be \n",
    "\n",
    "$$I(\\theta) =\\mathbb E\\left\\{ \\left[\\frac{\\partial}{\\partial \\theta}\\log f_\\theta(X)\\right] \\left[\\frac{\\partial}{\\partial \\theta}\\log f_\\theta(X)\\right] ^T\\right\\}.$$\n",
    "\n",
    "Here $\\frac{\\partial}{\\partial \\theta}\\log f_\\theta(X)$ is a column vector.\n",
    "\n",
    "When $\\frac{\\partial ^2}{\\partial \\theta_i\\theta_j }\\int f_\\theta (x)dx  = \\int \\frac{\\partial ^2}{\\partial \\theta_i\\partial \\theta_j} f_\\theta (x)dx$ for arbitrary indices $i,j$ (permission of interchanging differentiation and integral), we have identity\n",
    "\n",
    "$$I(\\theta) =-\\mathbb E\\left\\{ \\frac{\\partial^2}{\\partial \\theta\\partial \\theta^T}\\log f_\\theta(X)\\right\\}.$$\n",
    "\n",
    "**Proof** We focus on the $(i,j)$ entry of $I_(\\theta)$:\n",
    "\n",
    "$$\\begin{aligned}I_{i,j}(\\theta)  &= \\int  \\frac{\\partial}{\\partial \\theta_i}\\log f_\\theta(x)\\cdot \\frac{\\partial}{\\partial \\theta_j}\\log f_\\theta(x) \\cdot f_\\theta (x)dx= \\int \\frac{ \\frac{\\partial}{\\partial \\theta_i} f_\\theta(x)\\cdot \\frac{\\partial}{\\partial \\theta_j} f_\\theta(x)}{f^2_\\theta(x)}f_\\theta(x) dx\n",
    "\\\\ &=  \\int - \\frac{f_\\theta(x) \\frac{\\partial ^2}{\\partial \\theta_i\\partial \\theta_j}f_\\theta(x) - \\frac{\\partial}{\\partial \\theta_i} f_\\theta(x)\\cdot \\frac{\\partial}{\\partial \\theta_j} f_\\theta(x)}{f^2_\\theta(x)}f_\\theta(x) dx+\\int  \\frac{ f_\\theta(x)\\frac{\\partial ^2}{\\partial \\theta_i\\partial \\theta_j}f_\\theta(x) }{f^2_\\theta(x)}f_\\theta(x)dx.\\end{aligned}$$\n",
    "\n",
    "Observe $\\frac{\\partial^2\\log f_\\theta(x)}{\\partial \\theta_i\\partial \\theta_j} = \\frac{f_\\theta(x) \\frac{\\partial ^2}{\\partial \\theta_i\\partial \\theta_j}f_\\theta(x)- \\frac{\\partial}{\\partial \\theta_i} f_\\theta(x)\\cdot \\frac{\\partial}{\\partial \\theta_j} f_\\theta(x)}{f_\\theta(x)}$ in the first term. And also $\\int  \\frac{ f_\\theta(x)\\frac{\\partial ^2}{\\partial \\theta_i\\partial \\theta_j}f_\\theta(x) }{f^2_\\theta(x)}f_\\theta(x)dx\n",
    "= \\frac{\\partial ^2}{\\partial \\theta_i\\theta_j }\\int f_\\theta (x)dx = \\frac{\\partial ^2}{\\partial \\theta_i\\theta_j }1 = 0$ for the second term. We conclude the result $I(\\theta) =-\\mathbb E\\left\\{ \\frac{\\partial^2}{\\partial \\theta\\partial \\theta^T}\\log f_\\theta(X)\\right\\}$.\n",
    "\n",
    "#### Change of Variable\n",
    "\n",
    "If $\\theta = \\psi(\\eta)$ is a function of $\\eta$ and $\\psi$ is differentiable, then the Fisher information of $\\eta$ is given by \n",
    "\n",
    "$$I_\\eta =  \\left[\\frac{\\partial \\psi}{\\partial \\eta}\\right] I_\\theta \\left[\\frac{\\partial \\psi}{\\partial \\eta}\\right]^T.$$\n",
    "\n",
    "<br>\n",
    "\n",
    "### Cramér-Rao Lower Bound\n",
    "\n",
    "**Theorem** Let $X = (X_1,\\dotsc,X_n)$ be a sample from $\\mathbb P_\\theta$ where $\\mathbb P_\\theta$ is a member of the parametric family $\\mathcal P$. Suppose that $T(X)$ is an estimator with expectance $\\mathbb E(T(X)) =\\mathbb E(T_{\\mathbb P_\\theta}(X))= g(\\theta)$. When $g$ is differentiable and each $\\mathbb P_\\theta$ has p.d.f. $f_\\theta$ that allows interchanging differentiation and integral:\n",
    "$$\\frac{\\partial}{\\partial \\theta}\\int h(x)f_\\theta (x)dx =\\int h(x) \\frac{\\partial}{\\partial \\theta}f_\\theta (x)dx\\quad\\quad \\theta\\in \\Theta$$\n",
    "for both $h(x) \\equiv 1$ and $h(x) = T(x)$. Also, assume the Fisher information matrix $I(\\theta)$ is strictly positive definite for all $\\theta$. Then, we have the following bound\n",
    "$${\\rm Var}(T(X)) \\geqslant \\left[\\frac{\\partial g}{\\partial \\theta}\\right]^T[I(\\theta)]^{-1}\\left[\\frac{\\partial g}{\\partial \\theta}\\right]\\quad\\quad\\theta\\in\\Theta.$$\n",
    "\n",
    "**Proof of univariate case** We will prove the case where $\\theta\\in\\mathbb R$ is univariate and the inequality becomes ${\\rm Var}(T(X))I(\\theta)\\geqslant [g'(\\theta)]^2$. Actually we will simply show that $I(\\theta) = {\\rm Var}(\\frac{\\partial }{\\partial \\theta }\\log f_\\theta)$ and $g'(\\theta) = {\\rm Cov}(T(X), \\frac{\\partial}{\\partial \\theta }\\log f_\\theta)$.\n",
    "\n",
    "Taking $h(x) \\equiv 1$ in the condition, we have \n",
    "\n",
    "$$\\mathbb E\\left\\{\\frac{\\partial}{\\partial \\theta }\\log f_\\theta\\right\\}\n",
    "= \\int \\frac{\\partial}{\\partial \\theta }\\log f_\\theta (x)\\cdot f_\\theta(x)dx\n",
    "= \\int \\frac{\\frac{\\partial f_\\theta (x)}{\\partial \\theta } }{f_\\theta(x)} \\cdot f_\\theta(x)dx\n",
    "= \\int \\frac{\\partial}{\\partial \\theta }f_\\theta (x) dx\n",
    "= \\frac{\\partial}{\\partial \\theta } \\int 1dx = 0.$$\n",
    "\n",
    "Thus, $I(\\theta) = E\\left\\{(\\frac{\\partial}{\\partial \\theta }\\log f_\\theta)^2\\right\\} = {\\rm Var}(\\frac{\\partial}{\\partial \\theta }\\log f_\\theta)$.\n",
    "\n",
    "Similarly, taking $h(x)\\equiv T(x)$ in the condition,\n",
    "\n",
    "$${\\rm Cov}\\left\\{T(X), \\frac{\\partial}{\\partial \\theta }\\log f_\\theta\\right\\} \n",
    "=\\int  (T(x) - g(\\theta))  \\cdot \\frac{\\partial}{\\partial \\theta }\\log f_\\theta(x)\\cdot f_\\theta(x)dx=\\int  (T(x) - g(\\theta))\\frac{\\partial f_\\theta(x)}{\\partial \\theta } dx =\\frac{\\partial}{\\partial \\theta } \\int   T(x)f_\\theta(x)dx = g'(\\theta).$$\n",
    "\n",
    "Hence the theorem holds.\n",
    "\n",
    "<br>\n",
    "\n",
    "### Exponential Family\n",
    "\n",
    "Consider the exponential family $\\mathcal P$ with p.d.f. $f_\\theta(x) = h(x)\\exp\\{\\eta^T(\\theta) T(x) - \\xi(\\theta)\\}$. Assume $\\eta$ is a bijection and all the regularity conditions required are satisfied. Then the Fisher information for $\\eta(\\theta)$ is the variance-covariance matrix ${\\rm Var}(T(X))$. And the Fisher information for $\\mathbb E(T(X))$ is ${\\rm Var}(T(X))^{-1}$.\n",
    "\n",
    "**Proof** For $\\eta(\\theta)$, first we recall that we have proved $\\mathbb E(T(X)) = \\frac{\\partial \\xi(\\theta)}{\\partial \\eta}$ in the previous section (statistical property of GLM), so\n",
    "\n",
    "$$\\frac{\\partial \\log f}{\\partial \\eta} = T(x)  -\\frac{\\partial \\xi(\\theta)}{\\partial \\eta}\n",
    "=T(x) -\\mathbb E(T(X))\\quad\\Rightarrow\\quad I_\\eta = \\mathbb E\\left\\{[T(X) -\\mathbb E(T(X))][T(X) -\\mathbb E(T(X))]^T\\right\\} = {\\rm Var}(T(X)).$$\n",
    "\n",
    "For $\\mathbb E(T(X))$, denote $\\vartheta = \\mathbb E(T(X))=\\left. \\frac{\\partial \\xi(\\theta)}{\\partial \\eta}\\right|_{\\eta =(\\cdot)}$ to be a differentiable function of $\\eta$, and we have the identity\n",
    "\n",
    "$$I_\\eta  = \\left[\\frac{\\partial \\vartheta}{\\partial \\eta}\\right]I_{\\vartheta} \\left[\\frac{\\partial \\vartheta}{\\partial \\eta}\\right]^T\\quad\\Rightarrow\\quad I_{\\vartheta}   = \\left[\\frac{\\partial \\vartheta}{\\partial \\eta}\\right]^{-1} I_\\eta\\left[\\frac{\\partial \\vartheta}{\\partial \\eta}\\right]^{-T}.\n",
    "$$\n",
    "\n",
    "Note that $\\frac{\\partial \\vartheta}{\\partial \\eta}=\\frac{\\partial \\xi(\\theta)}{\\partial \\eta\\partial \\eta^T}$ and $I_\\eta = {\\rm Var}(T(X))$, it remains to show that $\\frac{\\partial \\xi(\\theta)}{\\partial \\eta\\partial \\eta^T} = {\\rm Var}(T(X))$. Actually this is also proved in the previous section of the property of GLM or in the chapter of exponential family."
   ]
  },
  {
   "attachments": {},
   "cell_type": "markdown",
   "metadata": {},
   "source": [
    "### Asymptotic Optimality"
   ]
  }
 ],
 "metadata": {
  "kernelspec": {
   "display_name": "Python 3.8.4 64-bit",
   "language": "python",
   "name": "python3"
  },
  "language_info": {
   "codemirror_mode": {
    "name": "ipython",
    "version": 3
   },
   "file_extension": ".py",
   "mimetype": "text/x-python",
   "name": "python",
   "nbconvert_exporter": "python",
   "pygments_lexer": "ipython3",
   "version": "3.8.4"
  },
  "orig_nbformat": 4,
  "vscode": {
   "interpreter": {
    "hash": "1120dc956da57eca5c948a0118f4cdcd4d1b3be98c72752ed298d16085a61d24"
   }
  }
 },
 "nbformat": 4,
 "nbformat_minor": 2
}
